Makefile
@@ -5,12 +5,14 @@
 all: misc.vo automata.vo
 
 doc: all 
-	coqdoc -d docs/html automata.v
+	coqdoc -d docs/html automata.v misc.v
 	mv docs/html/index.html docs/html/index.html.old
 	docs/undup.sh docs/html/index.html.old docs/html/index.html
 	rm docs/html/index.html.old
 	python2.6 docs/beautifier.py docs/html/automata.html > docs/html/automata.html.tmp
 	mv docs/html/automata.html.tmp docs/html/automata.html
+	python2.6 docs/beautifier.py docs/html/misc.html > docs/html/misc.html.tmp
+	mv docs/html/misc.html.tmp docs/html/misc.html
 
 clean:
 	rm -rf *.vo docs/*
